tidied up

peterson.dfy
@@ -14,73 +14,86 @@ ensures ValidProcess(q)
 }
 
 predicate Valid(s: State) {
-    (forall p :: p in s.flag.Keys && ValidProcess(p)) &&
-    (forall p :: p in s.pc.Keys && ValidProcess(p)) && 
-    (forall p :: ValidProcess(p) && (s.pc[p] == cs ==> (s.flag[p] && s.turn == p))) 
+    && (forall p :: p in s.flag.Keys && ValidProcess(p))
+    && (forall p :: p in s.pc.Keys && ValidProcess(p))
+    && (forall p :: ValidProcess(p) && (s.pc[p] == cs ==> (s.flag[p] && s.turn == p))) 
 }
 
-// predicate Init(s: State) {
-//     Valid(s) &&
-//     s.flag[0] == s.flag[1] == false &&
-//     s.turn == 0 &&
-//     s.pc[0] == a1 && s.pc[1] == a1
-// }
+predicate Init(s: State) {
+    && Valid(s)
+    && s.flag[0] == s.flag[1] == false
+    && s.turn == 0
+    && s.pc[0] == a1 && s.pc[1] == a1
+}
 
-// predicate Next(s: State, s': State) {
-//     Valid(s) &&
-//     exists p : Process :: ValidProcess(p) && NextP(p, s, s')
-// }
+predicate Next(s: State, s': State) {
+    && Valid(s)
+    && exists p : Process :: ValidProcess(p) && NextP(p, s, s')
+}
 
-// predicate NextP(p: Process, s: State, s': State)
-// requires Valid(s) && ValidProcess(p)
-// {
-//     (s.pc[p] == a1 && stmt_a1(p, s, s')) ||
-//     (s.pc[p] == a2 && stmt_a2(p, s, s')) ||
-//     (s.pc[p] == a3a && stmt_a3a(p, s, s')) ||
-//     (s.pc[p] == a3b && stmt_a3b(p, s, s')) ||
-//     (s.pc[p] == cs && stmt_cs(p, s, s')) ||
-//     (s.pc[p] == a4 && stmt_a4(p, s, s'))
-// }
+predicate NextP(p: Process, s: State, s': State)
+requires Valid(s) && ValidProcess(p)
+{
+    || (s.pc[p] == a1 && stmt_a1(p, s, s'))
+    || (s.pc[p] == a2 && stmt_a2(p, s, s'))
+    || (s.pc[p] == a3a && stmt_a3a(p, s, s'))
+    || (s.pc[p] == a3b && stmt_a3b(p, s, s'))
+    || (s.pc[p] == cs && stmt_cs(p, s, s'))
+    || (s.pc[p] == a4 && stmt_a4(p, s, s'))
+}
 
 predicate stmt_a1(p: Process, s: State, s': State) 
-requires ValidProcess(p) && Valid(s) && s.pc[p] == a1
+requires ValidProcess(p) && Valid(s)
 {
-    s'.flag == s.flag[p := true] &&
-    s'.pc == s.pc[p := a2]
+    && s.pc[p] == a1
+    && s'.flag == s.flag[p := true]
+    && s'.pc == s.pc[p := a2]
+    && s'.turn == s.turn
 }
 
 predicate stmt_a2(p: Process, s: State, s': State) 
-requires ValidProcess(p) && Valid(s) && s.pc[p] == a2
+requires ValidProcess(p) && Valid(s)
 {
-    s'.turn == Other(p) &&
-    s'.pc == s.pc[p := a3a]
+    && s.pc[p] == a2
+    && s'.turn == Other(p) 
+    && s'.pc == s.pc[p := a3a]
+    && s'.flag == s.flag
 }
 
 predicate stmt_a3a(p: Process, s: State, s': State) 
-requires ValidProcess(p) && Valid(s) && s.pc[p] == a3a
+requires ValidProcess(p) && Valid(s)
 {
-    (s.flag[Other(p)] && s'.pc == s.pc[p := a3b]) ||
-    (!s.flag[Other(p)] && s'.pc == s.pc[p := cs])
+    && s.pc[p] == a3a
+    && ((s.flag[Other(p)] && s'.pc == s.pc[p := a3b]) || (!s.flag[Other(p)] && s'.pc == s.pc[p := cs]))
+    && s'.turn == s.turn
+    && s'.flag == s.flag
 }
 
 predicate stmt_a3b(p: Process, s: State, s': State) 
-requires ValidProcess(p) && Valid(s) && s.pc[p] == a3b
+requires ValidProcess(p) && Valid(s) 
 {
-    (s.turn == Other(p) && s'.pc == s.pc[p := a3a]) ||
-    (s.turn != Other(p) && s'.pc == s.pc[p := cs])
+    && s.pc[p] == a3b
+    && ((s.turn == Other(p) && s'.pc == s.pc[p := a3a]) || (s.turn != Other(p) && s'.pc == s.pc[p := cs]))
+    && s'.turn == s.turn
+    && s'.flag == s.flag
 }
 
 predicate stmt_cs(p:Process, s: State, s': State) 
-requires ValidProcess(p) && Valid(s) && s.pc[p] == cs
+requires ValidProcess(p) && Valid(s) 
 {
-    s'.pc == s.pc[p := a4]
+    && s.pc[p] == cs
+    && s'.pc == s.pc[p := a4]
+    && s'.turn == s.turn
+    && s'.flag == s.flag
 }
 
 predicate stmt_a4(p: Process, s: State, s': State) 
-requires ValidProcess(p) && Valid(s) && s.pc[p] == a4 
+requires ValidProcess(p) && Valid(s) 
 {
-    s'.flag == s.flag[p := false] &&
-    s'.pc == s.pc[p := a1]
+    && s.pc[p] == a4 
+    && s'.flag == s.flag[p := false]
+    && s'.pc == s.pc[p := a1]
+    && s'.turn == s.turn
 }
 
 // Mutual Exclusion
@@ -88,6 +101,14 @@ lemma MutualExclusion(s: State, p: Process, q: Process)
 requires Valid(s) && ValidProcess(p) && ValidProcess(q)
 requires s.pc[p] == cs && s.pc[q] == cs
 ensures p == q
+{
+
+}
+
+// Invariance
+lemma Invariance(s: State, s':State)
+ensures Init(s) ==> Valid(s)
+ensures Valid(s) && Next(s, s') ==> Valid(s')
 {
 
 }
